Example.thy
@@ -17,19 +17,11 @@ abbreviation \<Phi>\<^sub>0 where "\<Phi>\<^sub>0 \<equiv> [
 
 lemma "[], 0 \<Turnstile> [] \<triangleright> \<Phi>\<^sub>0"
 apply (heron_next_step)
-(*
-apply (rule instant_i, auto, solve_run_witness)
-  apply (rule sporadic_e2, solve_run_witness)
-  apply (rule sporadic_e1, solve_run_witness)
-  apply (rule implies_e2, solve_run_witness)
-*)
-apply (heron_next_step) print_facts
-(*
-apply (rule instant_i, auto, solve_run_witness)
-  apply (rule sporadic_e2, solve_run_witness)
-  apply (rule implies_e2, solve_run_witness)
-*)
+  ML_val\<open>print_run @{Isar.goal}\<close>
+apply (heron_next_step)
+  ML_val\<open>print_run @{Isar.goal}\<close>
+apply (heron_next_step)
+  ML_val\<open>print_run @{Isar.goal}\<close>
 by (heron_end)
-(* by (rule simulation_end, simp, solve_run_witness') *)
 
 end
